synth_term to be proof carrying

Surface/Term/Definition.lean
@@ -12,7 +12,7 @@ inductive Term : Type where
 | var : Nat -> Term
 | global : {n m p : Nat} -> String -> Vec Core.Ty n -> Vec Core.Ty m -> Fun.Vec Term p -> Term
 | appt : Term -> Core.Ty -> Term
-| app : Term -> Term -> Term
+| app : Term -> Term -> Core.Ty -> Term
 | lamt :  Core.Kind -> Term -> Term
 | lam : Core.Ty -> Term -> Term
 -- | «match» : (n : Nat) -> Ty -> Term -> Fun.Vec Term n -> Fun.Vec Term n -> Term -> Term
@@ -24,7 +24,7 @@ notation:70 "g`#" x "`•ᵤ" a "`•ₑ" b "`•ₜ" c => Term.global x a b c
 
 notation f " `•[" a "]" => Term.appt f a
 
-notation:70 f " `• " a:70 => Term.app f a
+notation:70 f " `• " a:70 " :: " τ:70 => Term.app f a τ
 -- notation f " ∘[" a "]" => Term.ctor2 (Ctor2Variant.app BaseKind.open) f a
 
 -- bind notation
@@ -39,8 +39,8 @@ protected def Term.repr (p : Nat) : (a : Term) -> Std.Format
 | .global (p := p) n τU τE as =>
   let as : Fun.Vec Std.Format p := λ i => Term.repr p (as i)
   "g`#" ++ n ++ " `•ᵤ " ++ (τU.repr max_prec) ++ " `•ₑ " ++ (τE.repr max_prec) ++ " `• " ++ as.to.foldl (·++·) Std.Format.nil
-| .app t1 t2 =>
-  Repr.addAppParen (Term.repr max_prec t1 ++ " • " ++ Term.repr p t2) p
+| .app t1 t2 τ =>
+  Repr.addAppParen (Term.repr max_prec t1 ++ " • " ++ (Term.repr p t2 ++ " : " ++ τ.repr max_prec)) p
 | .appt t1 t2 =>
   Repr.addAppParen (Term.repr max_prec t1 ++ " •" ++ Std.Format.sbracket (t2.repr p)) p
 | .lamt K t =>
@@ -67,7 +67,7 @@ instance instRepr_Term : Repr Term where
 def Term.size : Term -> Nat
 | var _ => 1
 | global _ _ _ as => as.to.length + 1
-| app t1 t2 => t1.size + t2.size + 1
+| app t1 t2 _ => t1.size + t2.size + 1
 | appt t1 _ => size t1 + 1
 | lamt _ t => size t + 1
 | lam _ t => size t + 1
